\section{Seminumerischer Austausch}
\supercite{plessow2012seminumerical}
	\subsection{Theorie}
	\begin{equation}
	K_{\mu\nu\kappa\lambda}=\left(\chi_\mu\chi_\lambda\vert\chi_\kappa\chi_\nu\right)\approx \sum_{g}^{N_{\textrm{g}}} X_{\mu g}X_{\lambda g}A_{\kappa\nu g}
	\end{equation}		
	
	\begin{equation}
	X_{\mu g}=w_g^{\frac{1}{2}}\chi_\mu(\vec{r}_g)
	\end{equation}
	
	\begin{equation}
	A_{\kappa\nu g}=A_{\kappa\nu}(\vec{r}_g)=\int \frac{1}{\vert\vec{r}_g-\vec{r}_2\vert}\chi_\kappa(\vec{r}_2)\chi_\nu(\vec{r}_2)\Diff3\vec{r}_2
	\end{equation}
	
	\begin{equation}
%	\begin{aligned}
	K_{\mu\nu}=\frac{1}{2}\sum_{\kappa\lambda}^{N_{\textrm{BF}}}D_{\kappa\lambda} \left(\chi_\mu\chi_\lambda\vert\chi_\kappa\chi_\nu\right)
	\approx\frac{1}{2}\sum_{g}^{N_{\textrm{GIT}}}X_{\mu g}\underbrace{\sum_\kappa^{N_{\textrm{BF}}}A_{\kappa\nu g}\underbrace{\sum_\lambda^{N_{\textrm{BF}}}D_{\kappa\lambda}X_{\lambda g}}_{F_{\kappa g}}}_{G_{\nu g}}
%	\end{aligned}
	\end{equation}
	
	\begin{equation}
	\begin{aligned}
	\left.\frac{\partial K_{\mu\nu}}{\partial B_\beta}\right\vert_{\vec{B}=0}=&K_{\mu\nu}^{B_\beta}\\
	=&\underbrace{\frac{1}{2}\sum_{\kappa\lambda}^{N_{\textrm{BF}}}D_{\kappa\lambda}^{B_\beta} \left(\chi_\mu^{\vec{B}=0}\chi_\lambda^{\vec{B}=0}\vert\chi_\kappa^{\vec{B}=0}\chi_\nu^{\vec{B}=0}\right)}_{=K_{\mu\nu}^{B_\beta}[D^{B_\beta}]}\\
	&\underbrace{+\frac{1}{2}\sum_{\kappa\lambda}^{N_{\textrm{BF}}}D_{\kappa\lambda} \underbrace{\left[\left(\overline{\chi_\mu\chi_\lambda}\vert\chi_\kappa^{\vec{B}=0}\chi_\nu^{\vec{B}=0}\right)_\beta+\left(\chi_\mu^{\vec{B}=0}\chi_\lambda^{\vec{B}=0}\vert\overline{\chi_\kappa\chi_\nu}\right)_\beta\right]}_{=K_{\mu\nu\kappa\lambda}^{B_\beta}}}_{=K_{\mu\nu}^{B_\beta}[D]}.
	\end{aligned}
	\end{equation}
	
	\begin{equation}
	\begin{aligned}
	\left(\overline{\chi_\mu\chi_\lambda}\vert\chi_\kappa^{\vec{B}=0}\chi_\nu^{\vec{B}=0}\right)_\beta=&\frac{\iu}{2c} \left(\left(\vec{R}_{\mu\lambda}\times\vec{r}_1\right)_\beta\chi_\mu^{\vec{B}=0}\chi_\lambda^{\vec{B}=0}\vert\chi_\kappa^{\vec{B}=0}\chi_\nu^{\vec{B}=0}\right)\\
	=&\frac{\iu}{2c}\left(\vec{R}_\mu\times\vec{R}_\lambda\right)_\beta\left(\chi_\mu^{\vec{B}=0}\chi_\lambda^{\vec{B}=0}\vert\chi_\kappa^{\vec{B}=0}\chi_\nu^{\vec{B}=0}\right)\\
	&+\frac{\iu}{2c}\left[\vec{R}_{\mu\lambda}\times\left(\vec{r}_\mu\chi_\mu^{\vec{B}=0}\chi_\lambda^{\vec{B}=0}\vert\chi_\kappa^{\vec{B}=0}\chi_\nu^{\vec{B}=0}\right)\right]_\beta
	\end{aligned}
	\end{equation}
		\begin{equation}
	\begin{aligned}
	\left(\chi_\mu^{\vec{B}=0}\chi_\lambda^{\vec{B}=0}\vert\overline{\chi_\kappa\chi_\nu}\right)_\beta=&\frac{\iu}{2c}\left(\vec{R}_\kappa\times\vec{R}_\nu\right)_\beta\left(\chi_\mu^{\vec{B}=0}\chi_\lambda^{\vec{B}=0}\vert\chi_\kappa^{\vec{B}=0}\chi_\nu^{\vec{B}=0}\right)\\
	&+\frac{\iu}{2c}\left[\vec{R}_{\kappa\nu}\times\left(\chi_\mu^{\vec{B}=0}\chi_\lambda^{\vec{B}=0}\vert\chi_\kappa^{\vec{B}=0}\vec{r}_\nu\chi_\nu^{\vec{B}=0}\right)\right]_\beta
	\end{aligned}
	\end{equation}
	
	\begin{equation}
	\begin{aligned}
	K_{\mu\nu\kappa\lambda}^{B_x}=&\frac{\iu}{2c}\left[(R_{\mu\nu\kappa\lambda})_x\left(\chi_\mu^{\vec{B}=0}\chi_\lambda^{\vec{B}=0}\vert\chi_\kappa^{\vec{B}=0}\chi_\nu^{\vec{B}=0}\right)\right.\\
	&+\left(R_{\mu\lambda}\right)_y\left(z_\mu\chi_\mu^{\vec{B}=0}\chi_\lambda^{\vec{B}=0}\vert\chi_\kappa^{\vec{B}=0}\chi_\nu^{\vec{B}=0}\right)-\left(R_{\mu\lambda}\right)_z\left(y_\mu\chi_\mu^{\vec{B}=0}\chi_\lambda^{\vec{B}=0}\vert\chi_\kappa^{\vec{B}=0}\chi_\nu^{\vec{B}=0}\right)\\
	&\left.+\left(R_{\kappa\nu}\right)_y\left(\chi_\mu^{\vec{B}=0}\chi_\lambda^{\vec{B}=0}\vert\chi_\kappa^{\vec{B}=0}z_\nu\chi_\nu^{\vec{B}=0}\right)-\left(R_{\kappa\nu}\right)_z\left(\chi_\mu^{\vec{B}=0}\chi_\lambda^{\vec{B}=0}\vert\chi_\kappa^{\vec{B}=0}y_\nu\chi_\nu^{\vec{B}=0}\right)\right]
	\end{aligned}
	\end{equation}
	
	\begin{equation}
	(R_{\mu\nu\kappa\lambda})_x=(R_\mu)_y(R_\lambda)_z-(R_\mu)_z(R_\lambda)_y+(R_\kappa)_y(R_\nu)_z-(R_\kappa)_z(R_\nu)_y
	\end{equation}	
	
	\begin{equation}
	\begin{aligned}
	K_{\mu\nu}^{B_\beta}[D]\approx\frac{1}{2}\sum_{g}^{N_{\textrm{GIT}}}&\left[X_{\mu g}(G_{\mu\nu g})_\beta^0-\left(\vec{X}_{\mu g}^+\times\vec{G}_{\mu\nu g}^{\,1}\right)_\beta-\left(\vec{X}_{\nu g}^+\times\vec{G}_{\mu\nu g}^{\,2}\right)_\beta\right]
	\end{aligned}
	\end{equation}
	
	\begin{equation}
	\begin{aligned}
	&(G_{\mu\nu g})_\alpha^0=\sum_\kappa^{N_{\textrm{BF}}}A_{\kappa\nu g}(F_{\mu\nu\kappa g})_\alpha^0\\
	&(G_{\mu\nu g})_\alpha^1=\sum_\kappa^{N_{\textrm{BF}}}A_{\kappa\nu g}(F_{\mu\kappa g})_\alpha^1\\
	&(G_{\mu\nu g})_\alpha^2=\sum_\lambda^{N_{\textrm{BF}}}A_{\lambda\mu g}(F_{\nu\lambda g})_\alpha^2
	\end{aligned}
	\end{equation}	
	
	\begin{equation}
	\begin{aligned}
	&(F_{\mu\nu\kappa g})_\alpha^0=\sum_\lambda^{N_{\textrm{BF}}}D_{\kappa\lambda}X_{\lambda g}(R_{\mu\nu\kappa\lambda})_\alpha\\
	&(F_{\mu\kappa g})_\alpha^1=\sum_\lambda^{N_{\textrm{BF}}}D_{\kappa\lambda}X_{\lambda g}(R_{\mu\lambda})_\alpha\\
	&(F_{\nu\lambda g})_\alpha^2=\sum_\kappa^{N_{\textrm{BF}}}D_{\kappa\lambda}X_{\kappa g}(R_{\kappa\nu})_\alpha
	\end{aligned}
	\end{equation}
	
	\begin{equation}
	\left(X_{\mu g}^+\right)_\alpha=w_g^{\frac{1}{2}}\alpha_\mu\chi_\mu(\vec{r}_g)
	\end{equation}
	
	\begin{equation}
	\begin{aligned}
	K_{\mu\nu}^{B_x}[D]\approx\frac{1}{2}\sum_{g}^{N_{\textrm{GIT}}}&\left[X_{\mu g}\sum_\kappa^{N_{\textrm{BF}}}A_{\kappa\nu g}\sum_\lambda^{N_{\textrm{BF}}}D_{\kappa\lambda}X_{\lambda g}(R_{\mu\nu\kappa\lambda})_x\right.\\
	+&\left(X_{\mu g}\right)_z\sum_\kappa^{N_{\textrm{BF}}}A_{\kappa\nu g}\sum_\lambda^{N_{\textrm{BF}}}D_{\kappa\lambda}X_{\lambda g}(R_{\mu\lambda})_y\\
	-&\left(X_{\mu g}\right)_y\sum_\kappa^{N_{\textrm{BF}}}A_{\kappa\nu g}\sum_\lambda^{N_{\textrm{BF}}}D_{\kappa\lambda}X_{\lambda g}(R_{\mu\lambda})_z\\
	+&\left(X_{\nu g}\right)_z\sum_\lambda^{N_{\textrm{BF}}}A_{\lambda\mu g}\sum_\kappa^{N_{\textrm{BF}}}D_{\kappa\lambda}X_{\kappa g}(R_{\kappa\nu})_y\\
	-&\left.\left(X_{\nu g}\right)_y\sum_\lambda^{N_{\textrm{BF}}}A_{\lambda\mu g}\sum_\kappa^{N_{\textrm{BF}}}D_{\kappa\lambda}X_{\kappa g}(R_{\kappa\nu})_z\right]
	\end{aligned}
	\end{equation}
